src/compiler_generic/toy_example/embedding/Generator_static.thy
@@ -45,15 +45,15 @@ begin
 subsection\<open>Giving an Input to Translate\<close>
 
 definition "Design =
- (let n = \<lambda>n1 n2. OclTyObj (OclTyCore_pre n1) (case n2 of None \<Rightarrow> [] | Some n2 \<Rightarrow> [[OclTyCore_pre n2]])
-    ; mk = \<lambda>n l. ocl_class_raw.make n l [] False in
-  [ mk (n \<langle>''Galaxy''\<rangle> None) [(\<langle>''sound''\<rangle>, OclTy_raw \<langle>''unit''\<rangle>), (\<langle>''moving''\<rangle>, OclTy_raw \<langle>''bool''\<rangle>)]
-  , mk (n \<langle>''Planet''\<rangle> (Some \<langle>''Galaxy''\<rangle>)) [(\<langle>''weight''\<rangle>, OclTy_raw \<langle>''nat''\<rangle>)]
-  , mk (n \<langle>''Person''\<rangle> (Some \<langle>''Planet''\<rangle>)) [(\<langle>''salary''\<rangle>, OclTy_raw \<langle>''int''\<rangle>)] ])"
+ (let n = \<lambda>n1 n2. ToyTyObj (ToyTyCore_pre n1) (case n2 of None \<Rightarrow> [] | Some n2 \<Rightarrow> [[ToyTyCore_pre n2]])
+    ; mk = \<lambda>n l. toy_class_raw.make n l [] False in
+  [ mk (n \<langle>''Galaxy''\<rangle> None) [(\<langle>''sound''\<rangle>, ToyTy_raw \<langle>''unit''\<rangle>), (\<langle>''moving''\<rangle>, ToyTy_raw \<langle>''bool''\<rangle>)]
+  , mk (n \<langle>''Planet''\<rangle> (Some \<langle>''Galaxy''\<rangle>)) [(\<langle>''weight''\<rangle>, ToyTy_raw \<langle>''nat''\<rangle>)]
+  , mk (n \<langle>''Person''\<rangle> (Some \<langle>''Planet''\<rangle>)) [(\<langle>''salary''\<rangle>, ToyTy_raw \<langle>''int''\<rangle>)] ])"
 
 definition "main =
- (let n = \<lambda>n1. OclTyObj (OclTyCore_pre n1) []
-    ; OclMult = \<lambda>m r. ocl_multiplicity.make [m] r [Set] in
+ (let n = \<lambda>n1. ToyTyObj (ToyTyCore_pre n1) []
+    ; ToyMult = \<lambda>m r. toy_multiplicity.make [m] r [Set] in
   write_file
    (compiler_env_config.extend
      (compiler_env_config_empty True None (oidInit (Oid 0)) Gen_only_design (None, False)
@@ -62,11 +62,11 @@ definition "main =
                                       ,[\<langle>''../Toy_Library''\<rangle>]
                                       ,\<langle>''../embedding/Generator_dynamic''\<rangle>) \<rparr>)
      ( L.map (META_class_raw Floor1) Design
-       @@@@ [ META_association (ocl_association.make
-                                  OclAssTy_association
-                                  (OclAssRel [ (n \<langle>''Person''\<rangle>, OclMult (Mult_star, None) None)
-                                             , (n \<langle>''Person''\<rangle>, OclMult (Mult_nat 0, Some (Mult_nat 1)) (Some \<langle>''boss''\<rangle>))]))
-          , META_flush_all OclFlushAll]
+       @@@@ [ META_association (toy_association.make
+                                  ToyAssTy_association
+                                  (ToyAssRel [ (n \<langle>''Person''\<rangle>, ToyMult (Mult_star, None) None)
+                                             , (n \<langle>''Person''\<rangle>, ToyMult (Mult_nat 0, Some (Mult_nat 1)) (Some \<langle>''boss''\<rangle>))]))
+          , META_flush_all ToyFlushAll]
      , None)))"
 
 subsection\<open>Statically Executing the Exportation\<close>
