src/compiler_generic/toy_example/embedding/core/Core_init.thy
@@ -78,34 +78,34 @@ definition "find_class_ass env =
     partition (let\<^sub>O\<^sub>C\<^sub>a\<^sub>m\<^sub>l f = \<lambda>class. ClassRaw_clause class = [] in
                \<lambda> META_class_raw Floor1 class \<Rightarrow> f class
                | META_association _ \<Rightarrow> True
-               | META_ass_class Floor1 (OclAssClass _ class) \<Rightarrow> f class
+               | META_ass_class Floor1 (ToyAssClass _ class) \<Rightarrow> f class
                | META_class_synonym _ \<Rightarrow> True
                | _ \<Rightarrow> False) (rev (D_input_meta env)) in
   ( L.flatten [l_class, List.map_filter (let\<^sub>O\<^sub>C\<^sub>a\<^sub>m\<^sub>l f = \<lambda>class. class \<lparr> ClassRaw_clause := [] \<rparr> in
                                        \<lambda> META_class_raw Floor1 c \<Rightarrow> Some (META_class_raw Floor1 (f c))
-                                       | META_ass_class Floor1 (OclAssClass ass class) \<Rightarrow> Some (META_ass_class Floor1 (OclAssClass ass (f class)))
+                                       | META_ass_class Floor1 (ToyAssClass ass class) \<Rightarrow> Some (META_ass_class Floor1 (ToyAssClass ass (f class)))
                                        | _ \<Rightarrow> None) l_all_meta]
   , L.flatten (L.map
-      (let\<^sub>O\<^sub>C\<^sub>a\<^sub>m\<^sub>l f = \<lambda>class. [ META_ctxt Floor1 (ocl_ctxt_ext [] (ClassRaw_name class) (ClassRaw_clause class) ()) ] in
+      (let\<^sub>O\<^sub>C\<^sub>a\<^sub>m\<^sub>l f = \<lambda>class. [ META_ctxt Floor1 (toy_ctxt_ext [] (ClassRaw_name class) (ClassRaw_clause class) ()) ] in
        \<lambda> META_class_raw Floor1 class \<Rightarrow> f class
-       | META_ass_class Floor1 (OclAssClass _ class) \<Rightarrow> f class
+       | META_ass_class Floor1 (ToyAssClass _ class) \<Rightarrow> f class
        | x \<Rightarrow> [x]) l_all_meta)))"
 
 definition "map_enum_syn l_enum l_syn =
- (\<lambda> OclTy_object (OclTyObj (OclTyCore_pre s) []) \<Rightarrow> 
-      if list_ex (\<lambda>syn. s \<triangleq> (case syn of OclClassSynonym n _ \<Rightarrow> n)) l_syn then
-        OclTy_class_syn s
-      else if list_ex (\<lambda>enum. s \<triangleq> (case enum of OclEnum n _ \<Rightarrow> n)) l_enum then
-        OclTy_enum s
+ (\<lambda> ToyTy_object (ToyTyObj (ToyTyCore_pre s) []) \<Rightarrow> 
+      if list_ex (\<lambda>syn. s \<triangleq> (case syn of ToyClassSynonym n _ \<Rightarrow> n)) l_syn then
+        ToyTy_class_syn s
+      else if list_ex (\<lambda>enum. s \<triangleq> (case enum of ToyEnum n _ \<Rightarrow> n)) l_enum then
+        ToyTy_enum s
       else
-        OclTy_object (OclTyObj (OclTyCore_pre s) [])
+        ToyTy_object (ToyTyObj (ToyTyCore_pre s) [])
   | x \<Rightarrow> x)"
 
 definition "arrange_ass with_aggreg with_optim_ass l_c l_enum =
    (let l_syn = List.map_filter (\<lambda> META_class_synonym e \<Rightarrow> Some e
                                  | _ \<Rightarrow> None) l_c
       ; l_class = List.map_filter (\<lambda> META_class_raw Floor1 cflat \<Rightarrow> Some cflat
-                                   | META_ass_class Floor1 (OclAssClass _ cflat) \<Rightarrow> Some cflat
+                                   | META_ass_class Floor1 (ToyAssClass _ cflat) \<Rightarrow> Some cflat
                                    | _ \<Rightarrow> None) l_c
       ; l_class = (* map classes: change the (enumeration) type of every attributes to 'raw'
                                 instead of the default 'object' type *)
@@ -115,24 +115,24 @@ definition "arrange_ass with_aggreg with_optim_ass l_c l_enum =
                       L.map (map_prod id (map_enum_syn l_enum l_syn))
                                (ClassRaw_own cflat) \<rparr>) l_class
     ; l_ass = List.map_filter (\<lambda> META_association ass \<Rightarrow> Some ass
-                                 | META_ass_class Floor1 (OclAssClass ass _) \<Rightarrow> Some ass
+                                 | META_ass_class Floor1 (ToyAssClass ass _) \<Rightarrow> Some ass
                                  | _ \<Rightarrow> None) l_c
-      ; OclMult = \<lambda>l set. ocl_multiplicity_ext l None set ()
+      ; ToyMult = \<lambda>l set. toy_multiplicity_ext l None set ()
       ; (l_class, l_ass0) = 
           if with_optim_ass then
             (* move from classes to associations:
                  attributes of object types
-                 + those constructed with at most 1 recursive call to OclTy_collection *)
+                 + those constructed with at most 1 recursive call to ToyTy_collection *)
             map_prod rev rev (List.fold
                   (\<lambda>c (l_class, l_ass).
                     let default = [Set]
-                      ; f = \<lambda>role t mult_out. \<lparr> OclAss_type = OclAssTy_native_attribute
-                                              , OclAss_relation = OclAssRel [(ClassRaw_name c, OclMult [(Mult_star, None)] default)
+                      ; f = \<lambda>role t mult_out. \<lparr> ToyAss_type = ToyAssTy_native_attribute
+                                              , ToyAss_relation = ToyAssRel [(ClassRaw_name c, ToyMult [(Mult_star, None)] default)
                                                                             ,(t, mult_out \<lparr> TyRole := Some role \<rparr>)] \<rparr>
                       ; (l_own, l_ass) =
-                        List.fold (\<lambda> (role, OclTy_object t) \<Rightarrow>
-                                          \<lambda> (l_own, l). (l_own, f role t (OclMult [(Mult_nat 0, Some (Mult_nat 1))] default) # l)
-                                   | (role, OclTy_collection mult (OclTy_object t)) \<Rightarrow>
+                        List.fold (\<lambda> (role, ToyTy_object t) \<Rightarrow>
+                                          \<lambda> (l_own, l). (l_own, f role t (ToyMult [(Mult_nat 0, Some (Mult_nat 1))] default) # l)
+                                   | (role, ToyTy_collection mult (ToyTy_object t)) \<Rightarrow>
                                           \<lambda> (l_own, l). (l_own, f role t mult # l)
                                    | x \<Rightarrow> \<lambda> (l_own, l). (x # l_own, l))
                                   (ClassRaw_own c)
@@ -148,7 +148,7 @@ definition "arrange_ass with_aggreg with_optim_ass l_c l_enum =
                  attributes of aggregation form *)
             map_prod rev rev (List.fold
             (\<lambda>ass (l_class, l_ass).
-              if OclAss_type ass = OclAssTy_aggregation then
+              if ToyAss_type ass = ToyAssTy_aggregation then
                 ( fold_max
                     (\<lambda> (cpt_to, (name_to, category_to)).
                       case TyRole category_to of
@@ -158,14 +158,14 @@ definition "arrange_ass with_aggreg with_optim_ass l_c l_enum =
                             if cl_name_to_string cflat \<triangleq> ty_obj_to_string name_from then
                               Some (cflat \<lparr> ClassRaw_own :=
                                               L.flatten [ ClassRaw_own cflat
-                                                           , [(role_to, let ty = OclTy_object name_to in
+                                                           , [(role_to, let ty = ToyTy_object name_to in
                                                                         if single_multip category_to then 
                                                                           ty
                                                                         else
-                                                                          OclTy_collection category_to ty)]] \<rparr>)
+                                                                          ToyTy_collection category_to ty)]] \<rparr>)
                             else None))
                      | _ \<Rightarrow> \<lambda>_. id)
-                    (OclAss_relation' ass)
+                    (ToyAss_relation' ass)
                     l_class
                 , l_ass)
               else
@@ -185,13 +185,13 @@ subsection\<open>Main Combinators for the Translation\<close>
 
 definition "start_map f = L.mapM (\<lambda>x acc. (f x, acc))"
 definition "start_map''' f fl = (\<lambda> env.
-  let design_analysis = D_ocl_semantics env
-    ; base_attr = (if design_analysis = Gen_only_design then id else L.filter (\<lambda> (_, OclTy_object (OclTyObj (OclTyCore _) _)) \<Rightarrow> False | _ \<Rightarrow> True))
+  let design_analysis = D_toy_semantics env
+    ; base_attr = (if design_analysis = Gen_only_design then id else L.filter (\<lambda> (_, ToyTy_object (ToyTyObj (ToyTyCore _) _)) \<Rightarrow> False | _ \<Rightarrow> True))
     ; base_attr' = (\<lambda> (l_attr, l_inh). (base_attr l_attr, L.map base_attr l_inh))
     ; base_attr'' = (\<lambda> (l_attr, l_inh). (base_attr l_attr, base_attr l_inh)) in
   start_map f (fl design_analysis base_attr base_attr' base_attr'') env)"
 definition "start_map'' f fl e = start_map''' f (\<lambda>_. fl) e"
-definition "start_map'''' f fl = (\<lambda> env. start_map f (fl (D_ocl_semantics env)) env)"
+definition "start_map'''' f fl = (\<lambda> env. start_map f (fl (D_toy_semantics env)) env)"
 
 definition "bootstrap_floor f_x l env =
  (let (l, env) = f_x l env
@@ -206,13 +206,13 @@ definition "bootstrap_floor f_x l env =
   ( if D_output_auto_bootstrap env then
       l
     else
-      META_boot_generation_syntax (Boot_generation_syntax (D_ocl_semantics env))
+      META_boot_generation_syntax (Boot_generation_syntax (D_toy_semantics env))
       # l_setup
   , env \<lparr> D_output_auto_bootstrap := True \<rparr> ))"
 
-definition "wrap_oclty x = \<open>\<cdot>\<close> @@ x"
-definition "Term_annot_ocl e s = Term_annot' e (wrap_oclty s)"
-definition "Term_oclset l = (case l of [] \<Rightarrow> Term_basic [\<open>Set{}\<close>] | _ \<Rightarrow> Term_paren \<open>Set{\<close> \<open>}\<close> (term_binop \<open>,\<close> l))"
+definition "wrap_toyty x = \<open>\<cdot>\<close> @@ x"
+definition "Term_annot_toy e s = Term_annot' e (wrap_toyty s)"
+definition "Term_toyset l = (case l of [] \<Rightarrow> Term_basic [\<open>Set{}\<close>] | _ \<Rightarrow> Term_paren \<open>Set{\<close> \<open>}\<close> (term_binop \<open>,\<close> l))"
 definition "Term_oid s = (\<lambda>Oid n \<Rightarrow> Term_basic [s @@ String.of_natural n])"
 
 subsection\<open>Preliminaries on: Enumeration\<close>
@@ -239,6 +239,6 @@ subsection\<open>Preliminaries on: Context\<close>
 
 definition "make_ctxt_free_var pref ctxt =
  (var_self # L.flatten [ L.map fst (Ctxt_fun_ty_arg ctxt)
-                          , if pref = OclCtxtPre then [] else [var_result] ])"
+                          , if pref = ToyCtxtPre then [] else [var_result] ])"
 
 end
