src/compiler_generic/toy_example/embedding/core/Floor1_access.thy
@@ -42,13 +42,13 @@ theory  Floor1_access
 imports Core_init
 begin
 
-definition "print_access_oid_uniq_gen Thy_def D_ocl_oid_start_upd def_rewrite =
+definition "print_access_oid_uniq_gen Thy_def D_toy_oid_start_upd def_rewrite =
   (\<lambda>expr env.
-      (\<lambda>(l, oid_start). (L.map Thy_def l, D_ocl_oid_start_upd env oid_start))
+      (\<lambda>(l, oid_start). (L.map Thy_def l, D_toy_oid_start_upd env oid_start))
       (let (l, (acc, _)) = fold_class (\<lambda>isub_name name l_attr l_inh _ _ cpt.
-         let l_inh = L.map (\<lambda> OclClass _ l _ \<Rightarrow> l) (of_inh l_inh) in
+         let l_inh = L.map (\<lambda> ToyClass _ l _ \<Rightarrow> l) (of_inh l_inh) in
          let (l, cpt) = L.mapM (L.mapM
-           (\<lambda> (attr, OclTy_object (OclTyObj (OclTyCore ty_obj) _)) \<Rightarrow>
+           (\<lambda> (attr, ToyTy_object (ToyTyObj (ToyTyCore ty_obj) _)) \<Rightarrow>
                                             (let\<^sub>O\<^sub>C\<^sub>a\<^sub>m\<^sub>l obj_oid = TyObj_ass_id ty_obj
                                                ; obj_name_from_nat = TyObjN_ass_switch (TyObj_from ty_obj) in \<lambda>(cpt, rbt) \<Rightarrow>
              let (cpt_obj, cpt_rbt) =
@@ -59,12 +59,12 @@ definition "print_access_oid_uniq_gen Thy_def D_ocl_oid_start_upd def_rewrite =
              , cpt_rbt))
             | _ \<Rightarrow> \<lambda>cpt. ([], cpt)))
            (l_attr # l_inh) cpt in
-         (L.flatten (L.flatten l), cpt)) (D_ocl_oid_start env, RBT.empty) expr in
+         (L.flatten (L.flatten l), cpt)) (D_toy_oid_start env, RBT.empty) expr in
        (L.flatten l, acc)))"
 definition "print_access_oid_uniq =
   print_access_oid_uniq_gen
     O.definition
-    (\<lambda>env oid_start. env \<lparr> D_ocl_oid_start := oid_start \<rparr>)
+    (\<lambda>env oid_start. env \<lparr> D_toy_oid_start := oid_start \<rparr>)
     (\<lambda>obj_name_from_nat _ isub_name attr cpt_obj.
       Definition (Term_rewrite
                    (Term_basic [print_access_oid_uniq_name obj_name_from_nat isub_name attr])
