src/compiler_generic/toy_example/embedding/core/Floor1_ctxt.thy
@@ -51,8 +51,8 @@ definition "print_ctxt = (\<lambda>ctxt. bootstrap_floor
     let ((env, l_isab_ty), l_isab) = print_ctxt_const ctxt env in
     (L.flatten [l_isab_ty, l_isab, l], env))
   [ META_all_meta_embedding (META_ctxt Floor2
-      (map_invariant (\<lambda>T_inv b (OclProp_ctxt n p) \<Rightarrow>
-                       T_inv b (OclProp_ctxt n (T_lambdas (Ctxt_param ctxt @@@@ [var_self]) p)))
+      (map_invariant (\<lambda>T_inv b (ToyProp_ctxt n p) \<Rightarrow>
+                       T_inv b (ToyProp_ctxt n (T_lambdas (Ctxt_param ctxt @@@@ [var_self]) p)))
                      (map_pre_post (\<lambda>pref ctxt. T_lambdas (make_ctxt_free_var pref ctxt))
                                    ctxt))) ])"
 
