src/compiler_generic/toy_example/embedding/meta_toy/Printer_Toy.thy
@@ -62,9 +62,9 @@ fun of_ctxt2_term_aux where "of_ctxt2_term_aux l e =
   | T_lambda s c \<Rightarrow> of_ctxt2_term_aux (s # l) c) e"
 definition "of_ctxt2_term = of_ctxt2_term_aux []"
 
-definition' \<open>of_ocl_ctxt _ (floor :: (* polymorphism weakening needed by code_reflect *)
+definition' \<open>of_toy_ctxt _ (floor :: (* polymorphism weakening needed by code_reflect *)
                                      String.literal) ctxt = 
- (let f_inv = \<lambda> T_inv b (OclProp_ctxt n s) \<Rightarrow> \<open>  %sInv %s : "%s"\<close>
+ (let f_inv = \<lambda> T_inv b (ToyProp_ctxt n s) \<Rightarrow> \<open>  %sInv %s : "%s"\<close>
               (if b then \<open>Existential\<close> else \<open>\<close>)
               (case n of None \<Rightarrow> \<open>\<close> | Some s \<Rightarrow> To_string s)
               (of_ctxt2_term s) in
@@ -88,9 +88,9 @@ definition' \<open>of_ocl_ctxt _ (floor :: (* polymorphism weakening needed by c
         (String_concat \<open>
 \<close>
           (L.map
-            (\<lambda> T_pp pref (OclProp_ctxt n s) \<Rightarrow> \<open>  %s %s: "%s"\<close>
-                (case pref of OclCtxtPre \<Rightarrow> \<open>Pre\<close>
-                            | OclCtxtPost \<Rightarrow> \<open>Post\<close>)
+            (\<lambda> T_pp pref (ToyProp_ctxt n s) \<Rightarrow> \<open>  %s %s: "%s"\<close>
+                (case pref of ToyCtxtPre \<Rightarrow> \<open>Pre\<close>
+                            | ToyCtxtPost \<Rightarrow> \<open>Post\<close>)
                 (case n of None \<Rightarrow> \<open>\<close> | Some s \<Rightarrow> To_string s)
                 (of_ctxt2_term s)
              | T_invariant inva \<Rightarrow> f_inv inva)
@@ -104,7 +104,7 @@ lemmas [code] =
   (* def *)
   Print.concatWith_def
   Print.of_ctxt2_term_def
-  Print.of_ocl_ctxt_def
+  Print.of_toy_ctxt_def
   (* fun *)
   Print.of_ctxt2_term_aux.simps
 
